src/trans/eliminate_inductive.v
@@ -1,0 +1,111 @@
+From Src Require Import TyDefs TransDefs.
+Import MonadNotations.
+
+Local Open Scope errst_scope.
+
+(*TODO: do log, axm, imp when we know types of
+  monads*)
+
+Definition log {A: Type} (acc: list decl) 
+  (x: lsymbol * A) : errorHashconsT decl (list decl) :=
+  let (ps, _) := x in
+  p1 <- create_param_decl ps;;
+  errst_ret (p1 :: acc).
+Definition axm (acc: list decl) (x: prsymbol * term_c) : 
+  errorHashconsT decl (list decl) :=
+  let (pr, f) := x in
+  p1 <- create_prop_decl Paxiom pr f ;;
+  errst_ret (p1 :: acc).
+Definition imp {A: Type} (acc: list decl) (x: A * list (prsymbol * term_c)) : 
+  errorHashconsT decl (list decl) :=
+  let (_, al) := x in
+  fold_left_errst axm al acc.
+
+Definition t_and_simp (t1 t2: term_c) : term_c.
+Admitted.
+(*TODO: non-typechecking versions of some API
+  functions - then we can avoid error monad.
+  We already know that things are well-typed*)
+Definition exi {A: Type} (vl: list term_c) (x: A * term_c) : 
+  errorHashconsT ty_c term_c :=
+  let fix descend (f: term_c) : errorHashconsT ty_c term_c :=
+    match t_node_of f with
+    | Tquant Tforall f =>
+      (*TODO: is t_view_quant OK or do we need to open?*)
+      let '(vl, tl, f) := t_view_quant f in
+      d <- (descend f);;
+      errst_lift2 (t_exists_close vl tl d)
+    | Tbinop Timplies g f =>
+      d <- (descend f);;
+      errst_lift2 (t_and g d) 
+    | Tapp _ tl =>
+      let marry acc v t := 
+        t1 <- (t_equ v t) ;;
+        errst_ret (t_and_simp acc t1) in
+      o <- fold_left2_errst marry t_true vl tl;;
+      match o with
+      | None => (*cannot happen w typechecking*) errst_ret f
+      | Some x => errst_ret x
+      end
+    | Tlet t tb =>
+      let (v, f) := t_view_bound tb in
+      d <- (descend f);;
+      t1 <- errst_lift2 (t_let_close v t d);;
+      errst_ret t1
+    | _ => errst_ret f (*cannot be reached*)
+    end
+    in
+  descend (snd x).
+
+(*This is a partial function in why3, we give a default val here*)
+(*Need errState version*)
+Definition map_join_left_errst {A B St: Type} (d: B) 
+  (map: A -> errState St B) (join: B -> B -> errState St B) 
+  (l: list A) : errState St B :=
+  match l with
+  | x :: xl => 
+    y <- (map x) ;;
+    fold_left_errst (fun acc x => 
+    l1 <- (map x) ;;
+    join acc l1) xl y 
+  | _ => errst_ret d
+  end.
+
+(*TODO: LOTS of monad stuff we would like to avoid*)
+Definition inv {A: Type} (acc: list decl) (x: lsymbol * list (A * term_c)) : 
+  errState (CoqBigInt.t * (hashcons_ty ty_c * hashcons_ty decl)) (list decl) :=
+  let (ps, al) := x in
+  vl <- errst_tup1 ((errst_lift1 (
+    st_list (map (create_vsymbol (id_fresh1 "z")) ps.(ls_args))))) ;;
+  let tl := map t_var vl in
+  hd <- errst_tup2 (errst_tup1 (ps_app ps tl));;
+  (*TODO: don't need errState but dont want other ma_join_fold*)
+  dj <- errst_tup2 (errst_tup1 (map_join_left_errst t_true (exi tl) (fun t1 t2 => errst_lift2 (t_or t1 t2)) 
+    al)) ;;
+  (*TODO: implement simplification*)
+  hsdj <- errst_lift2 (t_implies hd dj) ;;
+  ax <- errst_lift2 (t_forall_close vl nil hsdj) ;;
+  let nm := id_derive1 (ps.(ls_name).(id_string) ++ "_inversion"%string)%string ps.(ls_name) in
+  p <- errst_lift1 (st_lift1 (create_prsymbol nm));;
+  pd <- errst_tup2 (errst_tup2 (create_prop_decl Paxiom p ax));;
+  errst_ret (pd :: acc).
+
+Definition elim (d: decl) : 
+  errState (CoqBigInt.t * (hashcons_ty ty_c * hashcons_ty decl)) (list decl) :=
+  match d.(d_node) with
+  | Dind x =>
+    let il := snd x in
+    dl <- errst_tup2 (errst_tup2 (fold_left_errst log il nil)) ;;
+    dl <- errst_tup2 (errst_tup2 (fold_left_errst imp il dl)) ;;
+    dl <- fold_left_errst inv il dl ;;
+    errst_ret (rev dl)
+  | _ => errst_ret [d]
+  end.
+
+(*Lift to hashcons_full*)
+
+Definition elim_lift (d: decl) :
+  errState (CoqBigInt.t * TransDefs.hashcons_full) (list decl) :=
+  @errst_congr1 CoqBigInt.t (hashcons_ty ty_c * hashcons_ty decl) _ _ full_of_ty_d (elim d).
+
+Definition eliminate_inductive := TransDefs.decl_errst elim_lift None.
